proof/refine/ARM_HYP/CNodeInv_R.thy
@@ -5057,26 +5057,29 @@ context begin interpretation Arch . (*FIXME: arch-split*)
 
 crunch cteSwap
   for tcb_at[wp]: "tcb_at' t"
-crunch cteSwap
-  for sch[wp]: "\<lambda>s. P (ksSchedulerAction s)"
-crunch cteSwap
-  for inQ[wp]: "obj_at' (inQ d p) tcb"
-crunch cteSwap
-  for ksQ[wp]: "\<lambda>s. P (ksReadyQueues s)"
-crunch cteSwap
-  for sym[wp]: "\<lambda>s. sym_refs (state_refs_of' s)"
-crunch cteSwap
-  for sym_hyp[wp]: "\<lambda>s. sym_refs (state_hyp_refs_of' s)"
-crunch cteSwap
-  for cur[wp]: "\<lambda>s. P (ksCurThread s)"
-crunch cteSwap
-  for ksCurDomain[wp]: "\<lambda>s. P (ksCurDomain s)"
-crunch cteSwap
-  for ksDomSchedule[wp]: "\<lambda>s. P (ksDomSchedule s)"
-crunch cteSwap
-  for it[wp]: "\<lambda>s. P (ksIdleThread s)"
-crunch cteSwap
-  for tcbDomain_obj_at'[wp]: "obj_at' (\<lambda>tcb. x = tcbDomain tcb) t"
+  and sch[wp]: "\<lambda>s. P (ksSchedulerAction s)"
+  and inQ[wp]: "obj_at' (inQ d p) tcb"
+  and ksQ[wp]: "\<lambda>s. P (ksReadyQueues s)"
+  and sym[wp]: "\<lambda>s. sym_refs (state_refs_of' s)"
+  and sym_hyp[wp]: "\<lambda>s. sym_refs (state_hyp_refs_of' s)"
+  and cur[wp]: "\<lambda>s. P (ksCurThread s)"
+  and ksCurDomain[wp]: "\<lambda>s. P (ksCurDomain s)"
+  and it[wp]: "\<lambda>s. P (ksIdleThread s)"
+  and tcbDomain_obj_at'[wp]: "obj_at' (\<lambda>tcb. x = tcbDomain tcb) t"
+  and ksInterrupt[wp]: "\<lambda>s. P (ksInterruptState s)"
+  and ksArch[wp]: "\<lambda>s. P (ksArchState s)"
+  and typ_at'[wp]: "\<lambda>s. P (typ_at' T p s)"
+  and ksDomSchedule[wp]: "\<lambda>s. P (ksDomSchedule s)"
+  and ksDomScheduleIdx[wp]: "\<lambda>s. P (ksDomScheduleIdx s)"
+  and ksDomScheduleStart[wp]: "\<lambda>s. P (ksDomScheduleStart s)"
+  and ct_not_inQ[wp]: "ct_not_inQ"
+  and pspace_domain_valid[wp]: "pspace_domain_valid"
+  and vms'[wp]: "valid_machine_state'"
+  and st_tcb_at'[wp]: "st_tcb_at' P t"
+  and ksqsL2[wp]: "\<lambda>s. P (ksReadyQueuesL2Bitmap s)"
+  and ksqsL1[wp]: "\<lambda>s. P (ksReadyQueuesL1Bitmap s)"
+  and irq_states'[wp]: "valid_irq_states'"
+  and valid_arch_state'[wp]: "valid_arch_state'"
 
 lemma cteSwap_idle'[wp]:
   "\<lbrace>valid_idle'\<rbrace>
@@ -5219,7 +5222,7 @@ lemma cteSwap_invs'[wp]:
   \<lbrace>\<lambda>rv. invs'\<rbrace>"
   apply (simp add: invs'_def valid_state'_def pred_conj_def)
   apply (rule hoare_pre)
-   apply (wp hoare_vcg_conj_lift sch_act_wf_lift
+   apply (wp hoare_vcg_conj_lift sch_act_wf_lift valid_dom_schedule'_lift
              valid_queues_lift cur_tcb_lift
              valid_irq_node_lift irqs_masked_lift tcb_in_cur_domain'_lift
              ct_idle_or_in_cur_domain'_lift2)
@@ -5693,7 +5696,7 @@ lemma make_zombie_invs':
   apply (wp updateCap_ctes_of_wp sch_act_wf_lift valid_queues_lift cur_tcb_lift
             updateCap_iflive' updateCap_ifunsafe' updateCap_idle'
             valid_irq_node_lift ct_idle_or_in_cur_domain'_lift2
-            updateCap_untyped_ranges_zero_simple
+            updateCap_untyped_ranges_zero_simple valid_dom_schedule'_lift
        | simp split del: if_split)+
   apply (intro conjI[rotated])
 
@@ -8802,7 +8805,7 @@ lemma cteMove_invs' [wp]:
    apply ((rule hoare_vcg_conj_lift, (wp cteMove_ifunsafe')[1])
                   | rule hoare_vcg_conj_lift[rotated])+
       apply (unfold cteMove_def)
-      apply (wp cur_tcb_lift valid_queues_lift haskell_assert_inv
+      apply (wp cur_tcb_lift valid_queues_lift haskell_assert_inv valid_dom_schedule'_lift
                 sch_act_wf_lift ct_idle_or_in_cur_domain'_lift2 tcb_in_cur_domain'_lift)+
   apply clarsimp
   done
@@ -9035,7 +9038,7 @@ lemma updateCap_noop_invs:
   apply (rule hoare_pre)
    apply (wp updateCap_ctes_of_wp updateCap_iflive'
              updateCap_ifunsafe' updateCap_idle'
-             valid_irq_node_lift
+             valid_irq_node_lift valid_dom_schedule'_lift
              updateCap_noop_irq_handlers sch_act_wf_lift
              untyped_ranges_zero_lift)
   apply (clarsimp simp: cte_wp_at_ctes_of modify_map_apply)
