proof/refine/X64/Untyped_R.thy
@@ -1382,6 +1382,7 @@ crunch updateMDB, updateNewFreeIndex
   and cns'[wp]: "\<lambda>s. P (gsCNodes s)"
   and ksDomainTime[wp]: "\<lambda>s. P (ksDomainTime s)"
   and ksDomScheduleIdx[wp]: "\<lambda>s. P (ksDomScheduleIdx s)"
+  and ksDomScheduleStart[wp]: "\<lambda>s. P (ksDomScheduleStart s)"
   and ksWorkUnitsCompleted[wp]: "\<lambda>s. P (ksWorkUnitsCompleted s)"
   and ksMachineState[wp]: "\<lambda>s. P (ksMachineState s)"
   and ksArchState[wp]: "\<lambda>s. P (ksArchState s)"
@@ -1390,6 +1391,8 @@ crunch insertNewCap
   and norq[wp]: "\<lambda>s. P (ksReadyQueues s)"
   and ksIdleThread[wp]: "\<lambda>s. P (ksIdleThread s)"
   and ksDomSchedule[wp]: "\<lambda>s. P (ksDomSchedule s)"
+  and ksDomScheduleIdx[wp]: "\<lambda>s. P (ksDomScheduleIdx s)"
+  and ksDomScheduleStart[wp]: "\<lambda>s. P (ksDomScheduleStart s)"
   and ksCurDomain[wp]: "\<lambda>s. P (ksCurDomain s)"
   and ksCurThread[wp]: "\<lambda>s. P (ksCurThread s)"
   (wp: crunch_wps)
@@ -3700,6 +3703,7 @@ lemma updateFreeIndex_clear_invs':
       apply (simp add:updateCap_def)
       apply (wp irqs_masked_lift cur_tcb_lift ct_idle_or_in_cur_domain'_lift
                 hoare_vcg_disj_lift untyped_ranges_zero_lift getCTE_wp valid_bitmaps_lift
+                valid_dom_schedule'_lift
                | wp (once) hoare_use_eq[where f="gsUntypedZeroRanges"]
                | simp add: getSlotCap_def
                | simp add: cte_wp_at_ctes_of)+
@@ -5385,7 +5389,7 @@ lemma insertNewCap_invs':
    apply (wp insertNewCap_valid_pspace' sch_act_wf_lift
              cur_tcb_lift tcb_in_cur_domain'_lift sym_heap_sched_pointers_lift
              insertNewCap_valid_global_refs' valid_bitmaps_lift
-             valid_arch_state_lift'
+             valid_arch_state_lift' valid_dom_schedule'_lift
              valid_irq_node_lift insertNewCap_valid_irq_handlers)
   apply (clarsimp simp: cte_wp_at_ctes_of)
   apply (frule ctes_of_valid[rotated, where p=parent, OF valid_pspace_valid_objs'])
